Untyped_Arithmetic_Expressions.thy
@@ -6,36 +6,272 @@ begin
 
 chapter {* Untyped Arithmetic Expressions *}
 
-text {* The language of untyped arithmetic expressions contains the boolean constants @{text true}
-and @{text false}, the conditional expression @{text "if \<dots> then \<dots> else \<dots>"}, the numeric constant
-@{text zero}, the arithmetic operators successor (@{text succ}) and predecessor (@{text pred}) and a
-function @{text is_zero} that returns @{text true} when applied to @{text zero} and @{text false}
-when applied to some other number. An arbitrary natural number $n$ can be expressed by applying the
-@{text succ} operator $n$ times to @{text zero} (e.g. the number three is @{text "succ (succ (succ
-zero))"}).*}
+text {*
+The untyped arithmetic expressions language is the first one we formalize. It consists of boolean
+expressions, containing the constants \texttt{true} and \texttt{false} and conditionals as
+primitives, and natural numbers, containing the constant \texttt{zero}, the successor and
+predecessor functions and an operation to test equality with zero as primitives. Following the book,
+we start with a subset containing only the boolean expression and carry on with fully fledged
+arithmetic expressions.
+*}
 
-section {* Syntax *}
+section {* Booleans *}
 
-text {* The syntax of this language is represented by the @{term NBTerm} datatype \footnote{To
-prevent name clashes with the \emph{Isabelle} constants of the same name, the types and type
-constructors are prefix with @{text NB}, which stand for "Numeric and Booleans". Functions use a
-suffix for the same purpose.}. *}
+text {*
+The syntax of this language is defined, in the book, in the following way:
 
-text {* \label{untyped-arith-NBTerm}*}
-datatype NBTerm =
+\begin{verbatim}
+  t ::=
+    true                        constant true
+    false                       constant false
+    if t then t else t          conditional
+\end{verbatim}
+
+Its counterpart, using Isabelle/HOL's syntax, is the \texttt{bterm} datatype: \footnote{To prevent
+name clashes with Isabelle's predefined types and constants of the same name, our types and type
+constructors are prefixed with \texttt{b}, which stand for "booleans". Functions use a suffix for
+the same purpose.}
+*}
+
+datatype bterm =
+  BTrue |
+  BFalse |
+  BIf bterm bterm bterm
+
+text {*
+The semantics of the language is defined using the small-step operational semantics which consists
+of an evaluation relation that performs the smallest possible step toward the final value. For the
+booleans, the only values are the constants @{term BTrue} and @{term BFalse}. To describe those,
+the book uses the following notation:
+
+\begin{verbatim}
+  v ::=
+    true           true value
+    false          false value
+\end{verbatim}
+
+We translate this in Isabelle/HOL using an inductive definition:
+*}
+
+inductive is_value_B :: "bterm \<Rightarrow> bool" where
+  "is_value_B BTrue" |
+  "is_value_B BFalse"
+
+text {*
+The evaluation relation is concerned with the way a conditional expression will be reduced. The book
+uses the standard mathematical notation for inference rules:
+
+\begin{verbatim}
+if true then t2 else t3 --> t2
+
+if false then t2 else t3 --> t3
+
+                  t1 --> t1'
+------------------------------------------------
+if t1 then t2 else t3 --> if t1' then t2 else t3
+\end{verbatim}
+
+These rules translate easily into an other inductive definition:
+*}
+
+inductive eval1_B :: "bterm \<Rightarrow> bterm \<Rightarrow> bool" where
+  eval1_BIf_BTrue: "eval1_B (BIf BTrue t2 t3) t2" |
+  eval1_BIf_BFalse: "eval1_B (BIf BFalse t2 t3) t3" |
+  eval1_BIf: "eval1_B t1 t1' \<Longrightarrow> eval1_B (BIf t1 t2 t3) (BIf t1' t2 t3)"
+
+(*<*)
+(* Example of definition 3.5.3 *)
+
+lemma
+  assumes
+    s: "s = BIf BTrue BFalse BFalse" and
+    t: "t = BIf s BTrue BTrue" and
+    u: "u = BIf BFalse BTrue BTrue"
+  shows "eval1_B (BIf t BFalse BFalse) (BIf u BFalse BFalse)"
+proof -
+  have "eval1_B s BFalse" unfolding s by (rule eval1_BIf_BTrue)
+  hence "eval1_B t u" unfolding t u by (rule eval1_BIf)
+  thus ?thesis by (rule eval1_BIf)
+qed
+(*>*)
+
+(* subsubsection {* Theorem 3.5.4 *} *)
+
+text {*
+With those basic definitions, we can turn to the first interesting theorem: the determinacy of
+one-step evaluation. As in the book, it goes by induction over the evaluation of @{term t} to
+@{term t'}, followed by a case analysis:
+*}
+
+theorem eval_single_determinacy:
+  "eval1_B t t' \<Longrightarrow> eval1_B t t'' \<Longrightarrow> t' = t''"
+proof (induction t t' arbitrary: t'' rule: eval1_B.induct)
+  case (eval1_BIf_BTrue t1 t2)
+  thus ?case by (auto elim: eval1_B.cases)
+next
+  case (eval1_BIf_BFalse t1 t2)
+  thus ?case by (auto elim: eval1_B.cases)
+next
+  case (eval1_BIf t1 t1' t2 t3)
+  from eval1_BIf.prems eval1_BIf.hyps show ?case
+    by (auto dest: eval1_BIf.IH elim: eval1_B.cases)
+qed
+
+(* subsubsection {* Theorem 3.5.7 *} *)
+
+text {*
+We now formalize the concept of normal form, for which the book gives the following definition:
+
+\begin{quotation}
+  \noindent A term \texttt{t} is in \emph{normal form} if no evaluation rule applies to it --- i.e.,
+  if there is no \texttt{t'} such that \texttt{t $\to$ t'}.
+\end{quotation}
+
+Since this definition mainly introduce some standard terminologie for some property of terms with
+respect to the single-step evaluation relation, we translate it using a simple synonym definition:
+*}
+
+definition is_normal_form_B :: "bterm \<Rightarrow> bool" where
+  "is_normal_form_B t \<longleftrightarrow> (\<forall>t'. \<not> eval1_B t t')"
+
+text {*
+We follows by proving, using a simple case analysis, that every value is in normal form:
+*}
+
+theorem value_imp_normal_form:
+  "is_value_B t \<Longrightarrow> is_normal_form_B t"
+by (auto elim: is_value_B.cases eval1_B.cases simp: is_normal_form_B_def)
+
+(* subsubsection {* Theorem 3.5.8 *} *)
+
+text {*
+For this simple language, the converse is also true: every term in normal form is a value. Our proof
+follows the book and use contradiction, structural induction over @{term t} and case analysis over
+the possible values.
+*}
+
+theorem normal_form_imp_value:
+  "is_normal_form_B t \<Longrightarrow> is_value_B t"
+by (rule ccontr, induction t rule: bterm.induct)
+  (auto intro: eval1_B.intros is_value_B.intros elim: is_value_B.cases simp: is_normal_form_B_def)
+
+(* subsubsection {* Definition 3.5.9 *} *)
+
+text {*
+The one-step evaluation is a very useful representation of the semantic of a language, but it does
+not represent what really interests us: the final value of an evaluation. To this end, the book
+defines a multi-step evaluation relation based on the single-step one:
+
+\begin{quotation}
+  \noindent The \emph{multi-step evaluation} relation $\to^*$ is the reflexive, transitive closure
+  of one-step evaluation. That is, it is the smallest relation such that (1) if t $t \to t'$ then
+  $t \to^* t'$, (2) $t \to^* t$ for all $t$, and (3) if $t \to^* t'$ and $t' \to^* t''$, then
+  $t \to^* t''$.
+\end{quotation}
+
+A direct translation of this definition would lead to the following definition:
+*}
+
+inductive eval_direct :: "bterm \<Rightarrow> bterm \<Rightarrow> bool" where
+  e_once: "eval1_B t t' \<Longrightarrow> eval_direct t t'" |
+  e_self: "eval_direct t t" |
+  e_transitive: "eval_direct t t' \<Longrightarrow> eval_direct t' t'' \<Longrightarrow> eval_direct t t''"
+
+text {*
+But this definition is inconvenient for theorem proving because it requires to consider three cases
+for each induction on a evaluation relation. We chose to define the multi-step evaluation relation
+using a shape similar to a list of one-step evaluations. The inductive definition consists of a base
+case, the reflexive application, and of an inductive case where one step of evaluation is perfomed:
+*}
+
+inductive eval_B :: "bterm \<Rightarrow> bterm \<Rightarrow> bool" where
+  e_base: "eval_B t t" |
+  e_step: "eval1_B t t' \<Longrightarrow> eval_B t' t'' \<Longrightarrow> eval_B t t''"
+
+text {*
+We then prove that this reprentation is equivalent to the direct translation of the definition found
+in the book before to continue:
+*}
+
+lemma eval_B_once:
+  "eval1_B t t' \<Longrightarrow> eval_B t t'"
+by (simp add: eval_B.intros)
+
+lemma eval_B_transitive:
+  "eval_B t t' \<Longrightarrow> eval_B t' t'' \<Longrightarrow> eval_B t t''"
+by (induction t t' rule: eval_B.induct) (auto intro: eval_B.intros)
+
+lemma eval_direct_eq_eval_B:
+  "eval_direct = eval_B"
+proof ((rule ext)+, rule iffI)
+  fix t t'
+  assume "eval_direct t t'"
+  thus "eval_B t t'" by (auto intro: e_base elim: eval_direct.induct eval_B_once eval_B_transitive)
+next
+  fix t t'
+  assume "eval_B t t'"
+  thus "eval_direct t t'" by (auto intro: e_self dest!: e_once elim: eval_B.induct e_transitive)
+qed
+
+(* subsubsection {* Corollary 3.5.11 *} *)
+
+text {*
+The next theorem we consider is the uniqueness of normal form, which is a corollary of the
+determinacy of the single-step evaluation:
+*}
+
+corollary uniqueness_of_normal_form:
+  "eval_B t u \<Longrightarrow> eval_B t u' \<Longrightarrow> is_normal_form_B u \<Longrightarrow> is_normal_form_B u' \<Longrightarrow> u = u'"
+proof (induction t u rule: eval_B.induct)
+  case (e_base t)
+  thus ?case by (auto elim: eval_B.cases simp: is_normal_form_B_def)
+next
+  case (e_step t t' t'')
+  thus ?case by (metis eval_B.cases is_normal_form_B_def eval_single_determinacy)
+qed
+
+text {*
+The last theorem we consider is the termination of evaluation. To prove it, we must first add a
+helper lemma about the size of terms after evaluation, which was implicitly assumed in the book:
+*}
+
+(*<*)
+(* subsubsection {* Theorem 3.5.12 *} *)
+primrec size_B :: "bterm \<Rightarrow> nat" where
+  "size_B BTrue = 1" |
+  "size_B BFalse = 1" |
+  "size_B (BIf t1 t2 t3) = 1 + size_B t1 + size_B t2 + size_B t3"
+(*>*)
+
+lemma eval_once_size_B:
+  "eval1_B t t' \<Longrightarrow> size_B t > size_B t'"
+by (induction t t' rule: eval1_B.induct) simp_all
+
+theorem termination_of_evaluation:
+  "\<exists>t'. eval_B t t' \<and> is_normal_form_B t'"
+by (induction rule: measure_induct_rule[of size_B])
+  (metis e_base e_step eval_once_size_B is_normal_form_B_def)
+
+section {* Arithmetic Expressions *}
+
+text {*
+We now turn to the fully fledged arithmetic expression language. The syntax is defined in the same
+way as for booleans:
+*}
+
+datatype nbterm =
   NBTrue |
   NBFalse |
-  NBIf NBTerm NBTerm NBTerm |
+  NBIf nbterm nbterm nbterm |
   NBZero |
-  NBSucc NBTerm |
-  NBPred NBTerm |
-  NBIs_zero NBTerm
+  NBSucc nbterm |
+  NBPred nbterm |
+  NBIs_zero nbterm
 
-section {* Induction on Terms *}
+(*<*)
+(* subsubsection {* Definition 3.3.1 *} *)
 
-subsubsection {* Definition 3.3.1 *}
-
-primrec const_NB :: "NBTerm \<Rightarrow> NBTerm set" where
+primrec const_NB :: "nbterm \<Rightarrow> nbterm set" where
   "const_NB NBTrue = {NBTrue}" |
   "const_NB NBFalse = {NBFalse}" |
   "const_NB NBZero = {NBZero}" |
@@ -44,9 +280,9 @@ primrec const_NB :: "NBTerm \<Rightarrow> NBTerm set" where
   "const_NB (NBIs_zero t) = const_NB t" |
   "const_NB (NBIf t1 t2 t3) = const_NB t1 \<union> const_NB t2 \<union> const_NB t3"
 
-subsubsection {* Definition 3.3.2 *}
+(* subsubsection {* Definition 3.3.2 *} *)
 
-primrec size_NB :: "NBTerm \<Rightarrow> nat" where
+primrec size_NB :: "nbterm \<Rightarrow> nat" where
   "size_NB NBTrue = 1" |
   "size_NB NBFalse = 1" |
   "size_NB NBZero = 1" |
@@ -55,7 +291,7 @@ primrec size_NB :: "NBTerm \<Rightarrow> nat" where
   "size_NB (NBIs_zero t) = size_NB t + 1" |
   "size_NB (NBIf t1 t2 t3) = size_NB t1 + size_NB t2 + size_NB t3 + 1"
 
-primrec depth_NB :: "NBTerm \<Rightarrow> nat" where
+primrec depth_NB :: "nbterm \<Rightarrow> nat" where
   "depth_NB NBTrue = 1" |
   "depth_NB NBFalse = 1" |
   "depth_NB NBZero = 1" |
@@ -64,7 +300,7 @@ primrec depth_NB :: "NBTerm \<Rightarrow> nat" where
   "depth_NB (NBIs_zero t) = depth_NB t + 1" |
   "depth_NB (NBIf t1 t2 t3) = max (depth_NB t1) (max (depth_NB t2) (depth_NB t3)) + 1"
 
-subsubsection {* Lemma 3.3.3 *}
+(* subsubsection {* Lemma 3.3.3 *} *)
 
 lemma card_union_leq_sum_card: "card (A \<union> B) \<le> card A + card B"
   by (cases "finite A \<and> finite B") (simp only: card_Un_Int, auto)
@@ -85,305 +321,209 @@ proof (induction t)
   qed
 qed (simp_all add: le_SucI)
 
-subsubsection {* Theorem 3.3.4 *}
+(* subsubsection {* Theorem 3.3.4 *} *)
 
 theorems induct_depth = measure_induct_rule[of depth_NB]
 theorems induct_size = measure_induct_rule[of size_NB]
-theorems structural_induction = NBTerm.induct
+theorems structural_induction = nbterm.induct
 
-section {* Semantic Styles *}
+(*>*)
 
-text {* A language is defined by both it's syntax and semantic. In the previous section, we
-rigorously defined our syntax by describing which terms are available and how they can be composed.
-We now need to define the semantic that those terms express. In the context of a programming
-language, we are interested in the effect of running the program. Since we are working with purely
-functional languages, the only possible effect is the value to which an expression evaluates.
-Therefore, we must provide a definition of the possible values and of the evaluation rules that let
-reach such values. There are three different approaches to formally describe a semantics:
+text {*
+Values now consist either of booleans or numeric values, for which a separate inductive
+definition is given. Here is the definition as founded in the book:
 
-\begin{enumerate}
-  \item \emph{Operational semantics} models the language as an abstract machine, where each possible
-    term is a state and where a transition function describes, for each state, the next state to
-    which an evaluation of the term would lead. If there exists no such next state, we says that the
-    machine has halted and that the current state is the final result of the program. Such a final
-    state can either be a value --- i.e. that conveys a meaning --- or a stuck term whose meaning is
-    not defined.
+\begin{verbatim}
+  v ::=
+    true             true value
+    false            false value
+    nv               numeric value
+  nv ::=
+    0                zero value
+    succ nv          successor value
+\end{verbatim}
 
-    There are two different flavours of operational semantics, namely \emph{small-step} and
-    \emph{big-steps}. They differ in the way the transition function works. In the former, the
-    smallest possible transition is chosen --- i.e. the terms representing the source and
-    destination states will only differ in a small way. In the later, it is the biggest transition
-    that is chosen. This difference implies that, under the \emph{small-step semantics}, many
-    transitions could be required to reach a final state while, under the \emph{big-step semantics},
-    a single transition bings us directly to the final state.
-  \item \emph{Denotational semantics}
-  \item \emph{Axiomatic semantics}
-\end{enumerate}
+Our inductive definition is very similar, but contains explicit assumptions on the nature of
+\texttt{nv}. The book uses naming conventions which define letters such as \texttt{t} as
+always representing terms, letters such as \texttt{v} as always representing values and variants of
+\texttt{nv} as always representing numeric values. In our formalization, such implicit assumption is
+possible for \texttt{t} because Isabelle/HOL infers that @{term nberm} is the only type that could
+be place at this position. Since values and numerical values do not have a proper type but are a
+subset of terms, we must add assumptions to declare the nature of these variables:
 *}
 
-text {* Operational semantics is used exclusively in this book. [TAPL p.34] *}
-
-section {* Evaluation *}
-
-text {* Before to attack our fully fledge arithmetic expression language, we will consider boolean
-expressions alone. *}
-
-subsection {* Booleans *}
-
-text {* The syntax of the boolean expressions language subset have only three constructs. *}
-
-datatype_new BTerm =
-  BTrue |
-  BFalse |
-  BIf BTerm BTerm BTerm
-
-text {* Out of which two are values. *}
-
-inductive is_value_B :: "BTerm \<Rightarrow> bool" where
-  "is_value_B BTrue" |
-  "is_value_B BFalse"
-
-text {* And the single step evaluation can proceed as follow. *}
-
-inductive eval_once_B :: "BTerm \<Rightarrow> BTerm \<Rightarrow> bool" where
-  eval_once_BIf_BTrue: "eval_once_B (BIf BTrue t2 t3) t2" |
-  eval_once_BIf_BFalse: "eval_once_B (BIf BFalse t2 t3) t3" |
-  eval_once_BIf: "eval_once_B t1 t1' \<Longrightarrow> eval_once_B (BIf t1 t2 t3) (BIf t1' t2 t3)"
-
-(* Example of definition 3.5.3 *)
-
-lemma
-  assumes
-    s: "s = BIf BTrue BFalse BFalse" and
-    t: "t = BIf s BTrue BTrue" and
-    u: "u = BIf BFalse BTrue BTrue"
-  shows "eval_once_B (BIf t BFalse BFalse) (BIf u BFalse BFalse)"
-proof -
-  have "eval_once_B s BFalse" unfolding s by (rule eval_once_BIf_BTrue)
-  hence "eval_once_B t u" unfolding t u by (rule eval_once_BIf)
-  thus ?thesis by (rule eval_once_BIf)
-qed
-
-subsubsection {* Theorem 3.5.4 *}
-
-theorem eval_single_determinacy:
-  "eval_once_B t t' \<Longrightarrow> eval_once_B t t'' \<Longrightarrow> t' = t''"
-proof (induction t t' arbitrary: t'' rule: eval_once_B.induct)
-  case (eval_once_BIf_BTrue t1 t2)
-  thus ?case by (auto elim: eval_once_B.cases)
-next
-  case (eval_once_BIf_BFalse t1 t2)
-  thus ?case by (auto elim: eval_once_B.cases)
-next
-  case (eval_once_BIf t1 t1' t2 t3)
-  from eval_once_BIf.prems eval_once_BIf.hyps show ?case
-    by (auto dest: eval_once_BIf.IH elim: eval_once_B.cases)
-qed
-
-subsubsection {* Theorem 3.5.7 *}
-
-definition is_normal_form_B :: "BTerm \<Rightarrow> bool" where
-  "is_normal_form_B t \<longleftrightarrow> (\<forall>t'. \<not> eval_once_B t t')"
-
-theorem value_imp_normal_form:
-  "is_value_B t \<Longrightarrow> is_normal_form_B t"
-by (auto simp: is_normal_form_B_def elim: is_value_B.cases eval_once_B.cases)
-
-subsubsection {* Theorem 3.5.8 *}
-
-theorem normal_form_imp_value:
-  "is_normal_form_B t \<Longrightarrow> is_value_B t"
-by (rule ccontr, induction t rule: BTerm.induct)
-  (auto
-    intro: eval_once_B.intros is_value_B.intros
-    elim: is_value_B.cases
-    simp: is_normal_form_B_def)
-
-subsubsection {* Definition 3.5.9 *}
-
-inductive eval_B :: "BTerm \<Rightarrow> BTerm \<Rightarrow> bool" where
-  e_base: "eval_B t t" |
-  e_step: "eval_once_B t t' \<Longrightarrow> eval_B t' t'' \<Longrightarrow> eval_B t t''"
-
-lemma e_once:
-  "eval_once_B t t' \<Longrightarrow> eval_B t t'"
-  by (simp add: e_base e_step)
-
-lemma e_transitive:
-  "eval_B t t' \<Longrightarrow> eval_B t' t'' \<Longrightarrow> eval_B t t''"
-by (induction t t' rule: eval_B.induct) (auto intro: eval_B.intros)
-
-subsubsection {* Corollary 3.5.11 *}
-
-corollary uniqueness_of_normal_form:
-  "eval_B t u \<Longrightarrow> eval_B t u' \<Longrightarrow> is_normal_form_B u \<Longrightarrow> is_normal_form_B u' \<Longrightarrow> u = u'"
-proof (induction t u rule: eval_B.induct)
-  case (e_base t)
-  thus ?case by (auto elim: eval_B.cases simp: is_normal_form_B_def)
-next
-  case (e_step t t' t'')
-  thus ?case by (metis eval_B.cases is_normal_form_B_def eval_single_determinacy)
-qed
-
-
-(* Util *)
-
-primrec size_B :: "BTerm \<Rightarrow> nat" where
-  "size_B BTrue = 1" |
-  "size_B BFalse = 1" |
-  "size_B (BIf t1 t2 t3) = 1 + size_B t1 + size_B t2 + size_B t3"
-
-lemma eval_once_size_B:
-  "eval_once_B t t' \<Longrightarrow> size_B t > size_B t'"
-by (induction t t' rule: eval_once_B.induct) (simp_all)
-
-subsubsection {* Theorem 3.5.12 *}
-
-theorem eval_always_terminate:
-  "\<exists>t'. eval_B t t' \<and> is_normal_form_B t'"
-by (induction rule: measure_induct_rule[of size_B])
-  (metis e_base e_step eval_once_size_B is_normal_form_B_def)
-
-subsection {* Arithmetic Expressions *}
-
-text {* \label{untyped-arith-is_value} *}
-
-inductive is_numeric_value_NB :: "NBTerm \<Rightarrow> bool" where
+inductive is_numeric_value_NB :: "nbterm \<Rightarrow> bool" where
   "is_numeric_value_NB NBZero" |
   "is_numeric_value_NB nv \<Longrightarrow> is_numeric_value_NB (NBSucc nv)"
 
-inductive is_value_NB :: "NBTerm \<Rightarrow> bool" where
+inductive is_value_NB :: "nbterm \<Rightarrow> bool" where
   "is_value_NB NBTrue" |
   "is_value_NB NBFalse" |
   "is_numeric_value_NB nv \<Longrightarrow> is_value_NB nv"
 
-text {* \label{untyped-arith-eval_once} *}
+text {*
+The single-step evaluation relation is a superset of the one defined for booleans:
+*}
 
-inductive eval_once_NB :: "NBTerm \<Rightarrow> NBTerm \<Rightarrow> bool" where
-  eval_once_NBIf_NBTrue: "eval_once_NB (NBIf NBTrue t2 t3) t2" |
-  eval_once_NBIf_NBFalse: "eval_once_NB (NBIf NBFalse t2 t3) t3" |
-  eval_once_NBIf: "eval_once_NB t1 t1' \<Longrightarrow> eval_once_NB (NBIf t1 t2 t3) (NBIf t1' t2 t3)" |
-  eval_once_NBSucc: "eval_once_NB t t' \<Longrightarrow> eval_once_NB (NBSucc t) (NBSucc t')" |
-  eval_once_NBPred_NBZero: "eval_once_NB (NBPred NBZero) NBZero" |
-  eval_once_NBPred_NBSucc: "is_numeric_value_NB nv \<Longrightarrow> eval_once_NB (NBPred (NBSucc nv)) nv" |
-  eval_once_NBPred: "eval_once_NB t t' \<Longrightarrow> eval_once_NB (NBPred t) (NBPred t')" |
-  eval_once_NBIs_zero_NBZero: "eval_once_NB (NBIs_zero NBZero) NBTrue" |
-  eval_once_NBIs_zero_NBSucc: "is_numeric_value_NB nv \<Longrightarrow> eval_once_NB (NBIs_zero (NBSucc nv)) NBFalse" |
-  eval_once_NBIs_zero: "eval_once_NB t t' \<Longrightarrow> eval_once_NB (NBIs_zero t) (NBIs_zero t')"
+inductive eval1_NB :: "nbterm \<Rightarrow> nbterm \<Rightarrow> bool" where
+  eval1_NBIf_NBTrue: "eval1_NB (NBIf NBTrue t2 t3) t2" |
+  eval1_NBIf_NBFalse: "eval1_NB (NBIf NBFalse t2 t3) t3" |
+  eval1_NBIf: "eval1_NB t1 t1' \<Longrightarrow> eval1_NB (NBIf t1 t2 t3) (NBIf t1' t2 t3)" |
+  eval1_NBSucc: "eval1_NB t t' \<Longrightarrow> eval1_NB (NBSucc t) (NBSucc t')" |
+  eval1_NBPred_NBZero: "eval1_NB (NBPred NBZero) NBZero" |
+  eval1_NBPred_NBSucc: "is_numeric_value_NB nv \<Longrightarrow> eval1_NB (NBPred (NBSucc nv)) nv" |
+  eval1_NBPred: "eval1_NB t t' \<Longrightarrow> eval1_NB (NBPred t) (NBPred t')" |
+  eval1_NBIs_zero_NBZero: "eval1_NB (NBIs_zero NBZero) NBTrue" |
+  eval1_NBIs_zero_NBSucc: "is_numeric_value_NB nv \<Longrightarrow> eval1_NB (NBIs_zero (NBSucc nv)) NBFalse" |
+  eval1_NBIs_zero: "eval1_NB t t' \<Longrightarrow> eval1_NB (NBIs_zero t) (NBIs_zero t')"
 
-inductive eval_NB :: "NBTerm \<Rightarrow> NBTerm \<Rightarrow> bool" where
+text {*
+The multi-step evaluation relation and the definition normal form are exactly the
+same as for booleans:
+*}
+
+inductive eval_NB :: "nbterm \<Rightarrow> nbterm \<Rightarrow> bool" where
   eval_NB_base: "eval_NB t t" |
-  eval_NB_step: "eval_once_NB t t' \<Longrightarrow> eval_NB t' t'' \<Longrightarrow> eval_NB t t''"
+  eval_NB_step: "eval1_NB t t' \<Longrightarrow> eval_NB t' t'' \<Longrightarrow> eval_NB t t''"
 
-definition is_normal_form_NB :: "NBTerm \<Rightarrow> bool" where
-  "is_normal_form_NB t \<longleftrightarrow> (\<forall>t'. \<not> eval_once_NB t t')"
+definition is_normal_form_NB :: "nbterm \<Rightarrow> bool" where
+  "is_normal_form_NB t \<longleftrightarrow> (\<forall>t'. \<not> eval1_NB t t')"
 
+text {*
+The reason is that all the actual work is perfomed by the singl-step evaluation relation and these
+two definition are just a convenient notation.
+
+In the book, the second covering this fully fledge arithmetic expression language is mainly an
+explanation of the constructions not present in the boolean expression language and does not
+contains any theorems. Nevertheless, we decided to reprove, or disprove, the theorems introduced in
+the section on booleans.
+*}
+
+(*<*)
 (* Usefull lemmas *)
 
-lemma eval_once_NB_impl_eval_NB: "eval_once_NB t t' \<Longrightarrow> eval_NB t t'"
+lemma eval1_NB_impl_eval_NB: "eval1_NB t t' \<Longrightarrow> eval_NB t t'"
   by (simp add: eval_NB_step eval_NB_base)
 
 lemma eval_NB_transitive: "eval_NB t t' \<Longrightarrow> eval_NB t' t'' \<Longrightarrow> eval_NB t t''"
-by (induction t t' arbitrary: t'' rule: eval_NB.induct) (auto intro: eval_NB.intros)
+by (induction t t' rule: eval_NB.induct) (auto intro: eval_NB.intros)
 
-lemma not_eval_once_numeric_value: "is_numeric_value_NB nv \<Longrightarrow> eval_once_NB nv t \<Longrightarrow> P"
+lemma not_eval_once_numeric_value: "is_numeric_value_NB nv \<Longrightarrow> eval1_NB nv t \<Longrightarrow> P"
 by (induction nv arbitrary: t rule: is_numeric_value_NB.induct)
-  (auto elim: eval_once_NB.cases)
+  (auto elim: eval1_NB.cases)
 
-subsubsection {* Theorem 3.5.4 for Arithmetic Expressions *}
+(* subsubsection {* Theorem 3.5.4 for Arithmetic Expressions *} *)
+(*>*)
 
-theorem eval_once_NB_right_unique:
-  "eval_once_NB t t' \<Longrightarrow> eval_once_NB t t'' \<Longrightarrow> t' = t''"
-proof (induction t t' arbitrary: t'' rule: eval_once_NB.induct)
-  case (eval_once_NBIf_NBTrue t1 t2)
-  thus ?case by (auto elim: eval_once_NB.cases)
+text {*
+The determinacy of the single-step evaluation still holds:
+*}
+
+theorem eval1_NB_right_unique:
+  "eval1_NB t t' \<Longrightarrow> eval1_NB t t'' \<Longrightarrow> t' = t''"
+proof (induction t t' arbitrary: t'' rule: eval1_NB.induct)
+  case (eval1_NBIf_NBTrue t1 t2)
+  thus ?case by (auto elim: eval1_NB.cases)
 next
-  case (eval_once_NBIf_NBFalse t1 t2)
-  thus ?case by (auto elim: eval_once_NB.cases)
+  case (eval1_NBIf_NBFalse t1 t2)
+  thus ?case by (auto elim: eval1_NB.cases)
 next
-  case (eval_once_NBIf t1 t1' t2 t3)
-  from eval_once_NBIf.prems eval_once_NBIf.hyps show ?case
-    by (auto intro: eval_once_NB.cases dest: eval_once_NBIf.IH)
+  case (eval1_NBIf t1 t1' t2 t3)
+  from eval1_NBIf.prems eval1_NBIf.hyps show ?case
+    by (auto intro: eval1_NB.cases dest: eval1_NBIf.IH)
 next
-  case (eval_once_NBSucc t1 t2)
-  from eval_once_NBSucc.prems eval_once_NBSucc.IH show ?case
-    by (auto elim: eval_once_NB.cases)
+  case (eval1_NBSucc t1 t2)
+  from eval1_NBSucc.prems eval1_NBSucc.IH show ?case
+    by (auto elim: eval1_NB.cases)
 next
-  case eval_once_NBPred_NBZero
-  thus ?case by (auto intro: eval_once_NB.cases)
+  case eval1_NBPred_NBZero
+  thus ?case by (auto intro: eval1_NB.cases)
 next
-  case (eval_once_NBPred_NBSucc nv1)
-  from eval_once_NBPred_NBSucc.prems eval_once_NBPred_NBSucc.hyps show ?case
-    by (cases rule: eval_once_NB.cases)
+  case (eval1_NBPred_NBSucc nv1)
+  from eval1_NBPred_NBSucc.prems eval1_NBPred_NBSucc.hyps show ?case
+    by (cases rule: eval1_NB.cases)
       (auto intro: is_numeric_value_NB.intros elim: not_eval_once_numeric_value[rotated])
 next
-  case (eval_once_NBPred t1 t2)
-  from eval_once_NBPred.hyps eval_once_NBPred.prems show ?case
+  case (eval1_NBPred t1 t2)
+  from eval1_NBPred.hyps eval1_NBPred.prems show ?case
     by (auto
-      intro: eval_once_NBPred.IH is_numeric_value_NB.intros
-      elim: eval_once_NB.cases
+      intro: eval1_NBPred.IH is_numeric_value_NB.intros
+      elim: eval1_NB.cases
       dest: not_eval_once_numeric_value)
 next
-  case eval_once_NBIs_zero_NBZero
-  thus ?case by (auto intro: eval_once_NB.cases)
+  case eval1_NBIs_zero_NBZero
+  thus ?case by (auto intro: eval1_NB.cases)
 next
-  case (eval_once_NBIs_zero_NBSucc nv)
+  case (eval1_NBIs_zero_NBSucc nv)
   thus ?case
-    by (auto intro: eval_once_NB.cases not_eval_once_numeric_value is_numeric_value_NB.intros)
+    by (auto intro: eval1_NB.cases not_eval_once_numeric_value is_numeric_value_NB.intros)
 next
-  case (eval_once_NBIs_zero t1 t2)
-  from eval_once_NBIs_zero.prems eval_once_NBIs_zero.hyps show ?case
-    by (cases rule: eval_once_NB.cases)
+  case (eval1_NBIs_zero t1 t2)
+  from eval1_NBIs_zero.prems eval1_NBIs_zero.hyps show ?case
+    by (cases rule: eval1_NB.cases)
       (auto
-        elim: eval_once_NB.cases
-        intro: eval_once_NBIs_zero.IH is_numeric_value_NB.intros
+        elim: eval1_NB.cases
+        intro: eval1_NBIs_zero.IH is_numeric_value_NB.intros
         elim: not_eval_once_numeric_value[rotated])
 qed
 
-subsubsection {* Theorem 3.5.7 for Arithmetic Expressions *}
+(* subsubsection {* Theorem 3.5.7 for Arithmetic Expressions *} *)
+
+text {*
+Every values are in normal form:
+*}
 
 theorem value_imp_normal_form_NB:
   "is_value_NB t \<Longrightarrow> is_normal_form_NB t"
   by (auto
     intro: not_eval_once_numeric_value
-    elim: eval_once_NB.cases is_value_NB.cases
+    elim: eval1_NB.cases is_value_NB.cases
     simp: is_normal_form_NB_def)
 
-subsubsection {* Theorem 3.5.8 does not hold for Arithmetic Expressions *}
+(* subsubsection {* Theorem 3.5.8 does not hold for Arithmetic Expressions *} *)
+
+text {*
+But contrary to boolean expressions, some expressions that are in normal form are not values. An
+example of such term is @{term "NBSucc NBTrue"}.
+*}
 
 theorem not_normal_form_imp_value_NB:
   "\<exists>t. is_normal_form_NB t \<and> \<not> is_value_NB t" (is "\<exists>t. ?P t")
 proof
   have a: "is_normal_form_NB (NBSucc NBTrue)"
-    by (auto elim: eval_once_NB.cases simp: is_normal_form_NB_def)
+    by (auto elim: eval1_NB.cases simp: is_normal_form_NB_def)
   have b: "\<not> is_value_NB (NBSucc NBTrue)"
     by (auto elim: is_numeric_value_NB.cases simp: is_value_NB.simps)
   from a b show "?P (NBSucc NBTrue)" by simp
 qed
 
-subsubsection {* Corollary 3.5.11 for Arithmetic Expressions *}
+(* subsubsection {* Corollary 3.5.11 for Arithmetic Expressions *} *)
+
+text {*
+The uniqueness of normal form still holds:
+*}
 
 corollary uniqueness_of_normal_form_NB:
-  assumes
-    "eval_NB t u" and
-    "eval_NB t u'" and
-    "is_normal_form_NB u" and
-    "is_normal_form_NB u'"
-  shows "u = u'"
-using assms
+  "eval_NB t u \<Longrightarrow> eval_NB t u' \<Longrightarrow> is_normal_form_NB u \<Longrightarrow> is_normal_form_NB u' \<Longrightarrow> u = u'"
 proof (induction t u arbitrary: u' rule: eval_NB.induct)
   case (eval_NB_base t)
   thus ?case by (auto elim: eval_NB.cases simp: is_normal_form_NB_def)
 next
   case (eval_NB_step t1 t2 t3)
-  thus ?case by (metis eval_NB.cases is_normal_form_NB_def eval_once_NB_right_unique)
+  thus ?case by (metis eval_NB.cases is_normal_form_NB_def eval1_NB_right_unique)
 qed
 
-subsubsection {* Theorem 3.5.12 for Arithmetic Expressions *}
+(* subsubsection {* Theorem 3.5.12 for Arithmetic Expressions *} *)
 
+text {*
+So does the termination of the evaluation function:
+*}
+
+(*<*)
 lemma eval_once_size_NB:
-  "eval_once_NB t t' \<Longrightarrow> size_NB t > size_NB t'"
-by (induction t t' rule: eval_once_NB.induct) auto
+  "eval1_NB t t' \<Longrightarrow> size_NB t > size_NB t'"
+by (induction t t' rule: eval1_NB.induct) auto
+(*>*)
 
 theorem eval_NB_always_terminate:
   "\<exists>t'. eval_NB t t' \<and> is_normal_form_NB t'"
